@prefix : <http://metarelate.net/config#> .
@prefix owl: <http://www.w3.org/2002/07/owl#> .
@prefix rdf: <http://www.w3.org/1999/02/22-rdf-syntax-ns#> .
@prefix xml: <http://www.w3.org/XML/1998/namespace> .
@prefix xsd: <http://www.w3.org/2001/XMLSchema#> .
@prefix rdfs: <http://www.w3.org/2000/01/rdf-schema#> .
@base <http://metarelate.net/config> .

<http://metarelate.net/config> rdf:type owl:Ontology ;
                               
                               owl:versionIRI <http://metarelate.net/config/v0> .


#################################################################
#
#    Annotation properties
#
#################################################################




#################################################################
#
#    Datatypes
#
#################################################################




#################################################################
#
#    Object Properties
#
#################################################################


###  http://metarelate.net/config/PragmaConfigProperties

<http://metarelate.net/config/PragmaConfigProperties> rdf:type owl:ObjectProperty .



###  http://metarelate.net/config/ValidationConfigProperties

<http://metarelate.net/config/ValidationConfigProperties> rdf:type owl:ObjectProperty .



###  http://metarelate.net/config/appliesTo

<http://metarelate.net/config/appliesTo> rdf:type owl:ObjectProperty ;
                                         
                                         rdfs:comment "Specifies to which Terminology Entity (e.r. reigister) a constraint applies. Constraints are transitively propagated to contained entities, unless a clear command is encountered." ;
                                         
                                         rdfs:range <http://metarelate.net/config/TerminologyEntity> ;
                                         
                                         rdfs:subPropertyOf <http://metarelate.net/config/ValidationConfigProperties> ;
                                         
                                         rdfs:domain <http://metarelate.net/config/ValidationTypes> .



###  http://metarelate.net/config/authConfigProperty

<http://metarelate.net/config/authConfigProperty> rdf:type owl:ObjectProperty .



###  http://metarelate.net/config/generatesProperty

<http://metarelate.net/config/generatesProperty> rdf:type owl:ObjectProperty ;
                                                 
                                                 rdfs:comment """<x> generatesProperty <y> implies that for any satement:
a <x> b, a new statement a <y> p is generated.""" ;
                                                 
                                                 rdfs:subPropertyOf <http://metarelate.net/config/reasonerConfigProperty> .



###  http://metarelate.net/config/generatesType

<http://metarelate.net/config/generatesType> rdf:type owl:ObjectProperty ;
                                             
                                             rdfs:comment """<x> generatesType <y> implies that for any satement:
a rdf:type <x>, a new statement a rdf:type <y> is generated.""" ;
                                             
                                             rdfs:subPropertyOf <http://metarelate.net/config/reasonerConfigProperty> .



###  http://metarelate.net/config/hasAuthConfigType

<http://metarelate.net/config/hasAuthConfigType> rdf:type owl:ObjectProperty ;
                                                 
                                                 rdfs:comment "Specifies which kind of authorization system is in place. " ;
                                                 
                                                 rdfs:range <http://metarelate.net/config/AuthorizationSystem> ;
                                                 
                                                 rdfs:subPropertyOf <http://metarelate.net/config/authConfigProperty> .



###  http://metarelate.net/config/hasDefaultUserID

<http://metarelate.net/config/hasDefaultUserID> rdf:type owl:ObjectProperty ;
                                                
                                                rdfs:comment "Links an innstance to its default user." ;
                                                
                                                rdfs:domain <http://metarelate.net/config/Instance> .



###  http://metarelate.net/config/hasEffectOnCode

<http://metarelate.net/config/hasEffectOnCode> rdf:type owl:ObjectProperty ;
                                               
                                               rdfs:comment "Specifies which roles apply to this action. Roles specified via this properties are considered to apply to the code in a register (process requests are defined x register)." ;
                                               
                                               rdfs:domain <http://metarelate.net/config/Action> ;
                                               
                                               rdfs:range <http://metarelate.net/config/Role> ;
                                               
                                               rdfs:subPropertyOf <http://metarelate.net/config/processConfigurationProperty> .



###  http://metarelate.net/config/hasEffectOnReg

<http://metarelate.net/config/hasEffectOnReg> rdf:type owl:ObjectProperty ;
                                              
                                              rdfs:comment "Specifies which roles apply to this action. Roles specified via this properties are considered to apply to the register r (process requests are defined x register, but can apply independently to the register or the contained codes)." ;
                                              
                                              rdfs:subPropertyOf <http://metarelate.net/config/processConfigurationProperty> .



###  http://metarelate.net/config/hasPragma

<http://metarelate.net/config/hasPragma> rdf:type owl:ObjectProperty ;
                                         
                                         rdfs:comment "specifies a prgama operator to be executed during import, for a code or register." ;
                                         
                                         rdfs:subPropertyOf <http://metarelate.net/config/PragmaConfigProperties> .



###  http://metarelate.net/config/hasSymmetric

<http://metarelate.net/config/hasSymmetric> rdf:type owl:ObjectProperty ;
                                            
                                            rdfs:comment "Specifes a symmetric property for the property object of this validation. Currently unimplemeneted, this could be used to automatically generate symmetric relations." ;
                                            
                                            rdfs:subPropertyOf <http://metarelate.net/config/ValidationConfigProperties> ;
                                            
                                            rdfs:domain <http://metarelate.net/config/ValidationTypes> .



###  http://metarelate.net/config/hasType

<http://metarelate.net/config/hasType> rdf:type owl:ObjectProperty ;
                                       
                                       rdfs:comment "Specifies types restrictions for a (data) property." ;
                                       
                                       rdfs:range <http://metarelate.net/config/DataTypes> ;
                                       
                                       rdfs:subPropertyOf <http://metarelate.net/config/ValidationConfigProperties> ;
                                       
                                       rdfs:domain <http://metarelate.net/config/ValidationTypes> .



###  http://metarelate.net/config/inRegister

<http://metarelate.net/config/inRegister> rdf:type owl:ObjectProperty ;
                                          
                                          rdfs:comment "The object of the specified (obejct) property must be contained in the specified register." ;
                                          
                                          rdfs:subPropertyOf <http://metarelate.net/config/ValidationConfigProperties> ;
                                          
                                          rdfs:domain <http://metarelate.net/config/ValidationTypes> .



###  http://metarelate.net/config/onDataProperty

<http://metarelate.net/config/onDataProperty> rdf:type owl:ObjectProperty ;
                                              
                                              rdfs:comment "the validation rules applies to the specified property (which is intended as a data property" ;
                                              
                                              rdfs:subPropertyOf <http://metarelate.net/config/ValidationConfigProperties> .



###  http://metarelate.net/config/onObjectProperty

<http://metarelate.net/config/onObjectProperty> rdf:type owl:ObjectProperty ;
                                                
                                                rdfs:comment "the validation rules applies to the specified property (which is intended as an object property)" ;
                                                
                                                rdfs:subPropertyOf <http://metarelate.net/config/ValidationConfigProperties> ;
                                                
                                                rdfs:domain <http://metarelate.net/config/ValidationTypes> .



###  http://metarelate.net/config/oneOf

<http://metarelate.net/config/oneOf> rdf:type owl:ObjectProperty ;
                                     
                                     rdfs:comment "the object of the (object) property must be one of the elements specified in the oneOf clauses (several can be repeated)." ;
                                     
                                     rdfs:subPropertyOf <http://metarelate.net/config/ValidationConfigProperties> .



###  http://metarelate.net/config/overrideProp

<http://metarelate.net/config/overrideProp> rdf:type owl:ObjectProperty ;
                                            
                                            rdfs:comment """A property to be overridden in a pragma expansion.
E.g.: 
entity/1-10 skos:notation 1-10

if the programa ovverideProp skos:notation,
entities are going to be expanded as follows:
entity/1 skos:notation 1
entity/2 skos:notation 2
...

(instead of, e.g.: entity/1 skos:notation 1-10)

""" ;
                                            
                                            rdfs:domain <http://metarelate.net/config/ExpandDashAndSuppress> ;
                                            
                                            rdfs:subPropertyOf <http://metarelate.net/config/PragmaConfigProperties> .



###  http://metarelate.net/config/postAux

<http://metarelate.net/config/postAux> rdf:type owl:ObjectProperty ;
                                       
                                       rdfs:comment "The resulting state of an auxiliary entitity (e.g.: a superseding term)" ;
                                       
                                       rdfs:domain <http://metarelate.net/config/Role> ;
                                       
                                       rdfs:range <http://metarelate.net/config/State> ;
                                       
                                       rdfs:subPropertyOf <http://metarelate.net/config/processConfigurationProperty> .



###  http://metarelate.net/config/postDown

<http://metarelate.net/config/postDown> rdf:type owl:ObjectProperty ;
                                        
                                        rdfs:comment "The resulting state for the children of the entity (how this varies respect to individual states is undefined)." ;
                                        
                                        rdfs:domain <http://metarelate.net/config/Role> ;
                                        
                                        rdfs:range <http://metarelate.net/config/State> ;
                                        
                                        rdfs:subPropertyOf <http://metarelate.net/config/processConfigurationProperty> .



###  http://metarelate.net/config/postThis

<http://metarelate.net/config/postThis> rdf:type owl:ObjectProperty ;
                                        
                                        rdfs:comment "the resulting state for the entity." ;
                                        
                                        rdfs:domain <http://metarelate.net/config/Role> ;
                                        
                                        rdfs:range <http://metarelate.net/config/State> ;
                                        
                                        rdfs:subPropertyOf <http://metarelate.net/config/processConfigurationProperty> .



###  http://metarelate.net/config/postUp

<http://metarelate.net/config/postUp> rdf:type owl:ObjectProperty ;
                                      
                                      rdfs:comment "The resulting state for the container of the entity" ;
                                      
                                      rdfs:domain <http://metarelate.net/config/Role> ;
                                      
                                      rdfs:range <http://metarelate.net/config/State> ;
                                      
                                      rdfs:subPropertyOf <http://metarelate.net/config/processConfigurationProperty> .



###  http://metarelate.net/config/pragmaProp

<http://metarelate.net/config/pragmaProp> rdf:type owl:ObjectProperty ;
                                          
                                          rdfs:domain <http://metarelate.net/config/ExpandDashAndSuppress> ;
                                          
                                          rdfs:range <http://metarelate.net/config/Parameter> ;
                                          
                                          rdfs:subPropertyOf <http://metarelate.net/config/PragmaConfigProperties> .



###  http://metarelate.net/config/pragmaSchema

<http://metarelate.net/config/pragmaSchema> rdf:type owl:ObjectProperty ;
                                            
                                            rdfs:comment "The schema in which the tree sctructure should be expressed" ;
                                            
                                            rdfs:domain <http://metarelate.net/config/ExpandTreeProcedure> ;
                                            
                                            rdfs:subPropertyOf <http://metarelate.net/config/PragmaConfigProperties> .



###  http://metarelate.net/config/pragmaTreeCollection

<http://metarelate.net/config/pragmaTreeCollection> rdf:type owl:ObjectProperty ;
                                                    
                                                    rdfs:comment "The collection in which new entities should be created." ;
                                                    
                                                    rdfs:domain <http://metarelate.net/config/ExpandTreeProcedure> ;
                                                    
                                                    rdfs:subPropertyOf <http://metarelate.net/config/PragmaConfigProperties> .



###  http://metarelate.net/config/preAux

<http://metarelate.net/config/preAux> rdf:type owl:ObjectProperty ;
                                      
                                      rdfs:comment """Pre condition: the state that an auxiliary entity must be in for this role to be \"triggered\" (e.g.: the state of a superseding term).
Note that all states (preUp, preDown, preThis, preAux) are considered in AND. Non specified states are considered as always viable.""" ;
                                      
                                      rdfs:domain <http://metarelate.net/config/Role> ;
                                      
                                      rdfs:range <http://metarelate.net/config/State> ;
                                      
                                      rdfs:subPropertyOf <http://metarelate.net/config/processConfigurationProperty> .



###  http://metarelate.net/config/preDown

<http://metarelate.net/config/preDown> rdf:type owl:ObjectProperty ;
                                       
                                       rdfs:comment """Pre condition: the state that the children of the entity must be in for this role to be \"triggered\" (only makes sense for registers)
Note that all states (preUp, preDown, preThis, preAux) are considered in AND. Non specified states are considered as always viable.""" ;
                                       
                                       rdfs:domain <http://metarelate.net/config/Role> ;
                                       
                                       rdfs:range <http://metarelate.net/config/State> ;
                                       
                                       rdfs:subPropertyOf <http://metarelate.net/config/processConfigurationProperty> .



###  http://metarelate.net/config/preThis

<http://metarelate.net/config/preThis> rdf:type owl:ObjectProperty ;
                                       
                                       rdfs:comment """Pre condition: the state that the entity must be in for this role to be \"triggered\".
Note that all states (preUp, preDown, preThis, preAux) are considered in AND. Non specified states are considered as always viable.""" ;
                                       
                                       rdfs:domain <http://metarelate.net/config/Role> ;
                                       
                                       rdfs:range <http://metarelate.net/config/State> ;
                                       
                                       rdfs:subPropertyOf <http://metarelate.net/config/processConfigurationProperty> .



###  http://metarelate.net/config/preUp

<http://metarelate.net/config/preUp> rdf:type owl:ObjectProperty ;
                                     
                                     rdfs:comment """Pre condition: the state that the container of the entity must be in for this role to be \"triggered\".
Note that all states (preUp, preDown, preThis, preAux) are considered in AND. Non specified states are considered as always viable.""" ;
                                     
                                     rdfs:domain <http://metarelate.net/config/Role> ;
                                     
                                     rdfs:range <http://metarelate.net/config/State> ;
                                     
                                     rdfs:subPropertyOf <http://metarelate.net/config/processConfigurationProperty> .



###  http://metarelate.net/config/processConfigurationProperty

<http://metarelate.net/config/processConfigurationProperty> rdf:type owl:ObjectProperty ;
                                                            
                                                            rdfs:domain <http://metarelate.net/config/Action> ;
                                                            
                                                            rdfs:range <http://metarelate.net/config/Role> .



###  http://metarelate.net/config/propertyFocus

<http://metarelate.net/config/propertyFocus> rdf:type owl:ObjectProperty ;
                                             
                                             rdfs:comment "Whether a property pertains to a code or to the concept represented," ;
                                             
                                             rdfs:range <http://metarelate.net/config/PropertyFocus> .



###  http://metarelate.net/config/reasonerConfigProperty

<http://metarelate.net/config/reasonerConfigProperty> rdf:type owl:ObjectProperty .



###  http://metarelate.net/config/symmetric

<http://metarelate.net/config/symmetric> rdf:type owl:ObjectProperty ;
                                         
                                         rdfs:comment """<x> symmetrix <y> implies that for any statement:
a <x> b, a new statement b <y> a is generated (and vice versa).""" ;
                                         
                                         rdfs:subPropertyOf <http://metarelate.net/config/reasonerConfigProperty> .



###  http://metarelate.net/config/validationCommand

<http://metarelate.net/config/validationCommand> rdf:type owl:ObjectProperty ;
                                                 
                                                 rdfs:comment "Associated a validation command to a validation rule." ;
                                                 
                                                 rdfs:range <http://metarelate.net/config/ValidationCommands> ;
                                                 
                                                 rdfs:subPropertyOf <http://metarelate.net/config/ValidationConfigProperties> ;
                                                 
                                                 rdfs:domain <http://metarelate.net/config/ValidationTypes> .



###  http://metarelate.net/states/overrides

<http://metarelate.net/states/overrides> rdf:type owl:ObjectProperty ;
                                         
                                         rdfs:comment "Re-defines a system property or resource" .





#################################################################
#
#    Data properties
#
#################################################################


###  http://metarelate.net/config/baseURL

<http://metarelate.net/config/baseURL> rdf:type owl:DatatypeProperty ;
                                       
                                       rdfs:comment "The root of the server URL (after which the terminology server can append its bits). Note that this is a parameter and hence specified as a literal." ;
                                       
                                       rdfs:subPropertyOf <http://metarelate.net/config/systemParameters> .



###  http://metarelate.net/config/cssAddress

<http://metarelate.net/config/cssAddress> rdf:type owl:DatatypeProperty ;
                                          
                                          rdfs:comment "the location of a css file to be used for rendering (possibly obsolete in the the new rendering system)." ;
                                          
                                          rdfs:subPropertyOf <http://metarelate.net/config/systemParameters> .



###  http://metarelate.net/config/diskPrefix

<http://metarelate.net/config/diskPrefix> rdf:type owl:DatatypeProperty ;
                                          
                                          rdfs:comment "the directory where a file-based Linked-Data representation can be generated." ;
                                          
                                          rdfs:subPropertyOf <http://metarelate.net/config/systemParameters> .



###  http://metarelate.net/config/hardLimit

<http://metarelate.net/config/hardLimit> rdf:type owl:DatatypeProperty ;
                                         
                                         rdfs:comment """Specifies a limit for range expansions: e.g.: entity/1-100.
If an hardLimit of 20 is specified,  only entity/1....entity/20 are produced.
Unless hardLimitCut is specified via pragmaProp, in which case none is produced.""" ;
                                         
                                         rdfs:domain <http://metarelate.net/config/ExpandDashAndSuppress> ;
                                         
                                         rdfs:subPropertyOf <http://metarelate.net/config/pragmaDataProperty> .



###  http://metarelate.net/config/hasAuthDir

<http://metarelate.net/config/hasAuthDir> rdf:type owl:DatatypeProperty ;
                                          
                                          rdfs:comment "Specifies the directory where authorization files can be found (absolute path)"@en ;
                                          
                                          rdfs:subPropertyOf <http://metarelate.net/config/systemParameters> .



###  http://metarelate.net/config/hasCacheDir

<http://metarelate.net/config/hasCacheDir> rdf:type owl:DatatypeProperty ;
                                           
                                           rdfs:comment "Specifies the directory where cache files are found (absolute dirs)"@en ;
                                           
                                           rdfs:subPropertyOf <http://metarelate.net/config/systemParameters> .



###  http://metarelate.net/config/hasDBDir

<http://metarelate.net/config/hasDBDir> rdf:type owl:DatatypeProperty ;
                                        
                                        rdfs:comment "The location of the TDB in use by the system" ;
                                        
                                        rdfs:subPropertyOf <http://metarelate.net/config/systemParameters> .



###  http://metarelate.net/config/hasGitDir

<http://metarelate.net/config/hasGitDir> rdf:type owl:DatatypeProperty ;
                                         
                                         rdfs:comment "Specifies teh directory used for git support to distributed code management system (currently unimplemented)."@en ;
                                         
                                         rdfs:subPropertyOf <http://metarelate.net/config/systemParameters> .



###  http://metarelate.net/config/hasInstanceIdentifier

<http://metarelate.net/config/hasInstanceIdentifier> rdf:type owl:DatatypeProperty ;
                                                     
                                                     rdfs:comment "A unique string identifying an instance (usually a UUID)." ;
                                                     
                                                     rdfs:domain <http://metarelate.net/config/Instance> ;
                                                     
                                                     rdfs:subPropertyOf <http://metarelate.net/config/instanceDataProperties> .



###  http://metarelate.net/config/hasPdfLatexCommand

<http://metarelate.net/config/hasPdfLatexCommand> rdf:type owl:DatatypeProperty ;
                                                  
                                                  rdfs:comment "Speciefies where the pdflatex command can be found (absolute path)"@en ;
                                                  
                                                  rdfs:subPropertyOf <http://metarelate.net/config/systemParameters> .



###  http://metarelate.net/config/hasPrefixFile

<http://metarelate.net/config/hasPrefixFile> rdf:type owl:DatatypeProperty ;
                                             
                                             rdfs:comment "A files whose prefixes are  used in the rdf exports"@en ;
                                             
                                             rdfs:subPropertyOf <http://metarelate.net/config/systemParameters> .



###  http://metarelate.net/config/hasSeedFile

<http://metarelate.net/config/hasSeedFile> rdf:type owl:DatatypeProperty ;
                                           
                                           rdfs:comment "A file containing the identifier (seed) for this instance."@en ;
                                           
                                           rdfs:subPropertyOf <http://metarelate.net/config/systemParameters> .



###  http://metarelate.net/config/hasTemplatesDir

<http://metarelate.net/config/hasTemplatesDir> rdf:type owl:DatatypeProperty ;
                                               
                                               rdfs:comment "Specifies the directory where template files can be found (abosulte files). Files are grouped in sub-directory of the declared directory, named after the template name."@en ;
                                               
                                               rdfs:subPropertyOf <http://metarelate.net/config/systemParameters> .



###  http://metarelate.net/config/hasWebPackageDir

<http://metarelate.net/config/hasWebPackageDir> rdf:type owl:DatatypeProperty ;
                                                
                                                rdfs:comment "the directory where the WAR application for the admin interface can be found."@en ;
                                                
                                                rdfs:subPropertyOf <http://metarelate.net/config/systemParameters> .



###  http://metarelate.net/config/instanceDataProperties

<http://metarelate.net/config/instanceDataProperties> rdf:type owl:DatatypeProperty .



###  http://metarelate.net/config/language

<http://metarelate.net/config/language> rdf:type owl:DatatypeProperty ;
                                        
                                        rdfs:comment """the language for this property. Note that for cardinality counts, a property with a language specified is consider as a distinct property.
E.g.: myLabel with language \"en\" and myLabel withLnaguge \"fr\" are two distinct properties.
Object of thei property should be a two letter language code, as defiend in the RDF specs.""" ;
                                        
                                        rdfs:subPropertyOf <http://metarelate.net/config/validationDataProperties> .



###  http://metarelate.net/config/maxCardinality

<http://metarelate.net/config/maxCardinality> rdf:type owl:DatatypeProperty ;
                                              
                                              rdfs:comment "the maximum number of times this property can be asserted." ;
                                              
                                              rdfs:domain <http://metarelate.net/config/ValidationTypes> ;
                                              
                                              rdfs:subPropertyOf <http://metarelate.net/config/validationDataProperties> .



###  http://metarelate.net/config/minCardinality

<http://metarelate.net/config/minCardinality> rdf:type owl:DatatypeProperty ;
                                              
                                              rdfs:comment "the minimum number of times this property has to be asserted (0=optional)" ;
                                              
                                              rdfs:domain <http://metarelate.net/config/ValidationTypes> ;
                                              
                                              rdfs:subPropertyOf <http://metarelate.net/config/validationDataProperties> .



###  http://metarelate.net/config/overridesDiskPrefix

<http://metarelate.net/config/overridesDiskPrefix> rdf:type owl:DatatypeProperty ;
                                                   
                                                   rdfs:comment "Specifies an alternative directory that, for a specific action, can ovverride the system-wide diretcory used for a file-based linked-data representation. In use a configuration of the publication pipeline, subject to reworking." ;
                                                   
                                                   owl:deprecated "" ;
                                                   
                                                   rdfs:subPropertyOf <http://metarelate.net/config/systemParameters> .



###  http://metarelate.net/config/overridesSitePrefix

<http://metarelate.net/config/overridesSitePrefix> rdf:type owl:DatatypeProperty ;
                                                   
                                                   rdfs:comment "Specifies an alternative baseURL that can ovverride the system-wide baseURL for a specific action. In use a configuration of the publication pipeline, subject to reworking." ;
                                                   
                                                   owl:deprecated "" ;
                                                   
                                                   rdfs:subPropertyOf <http://metarelate.net/config/systemParameters> .



###  http://metarelate.net/config/pattern

<http://metarelate.net/config/pattern> rdf:type owl:DatatypeProperty ;
                                       
                                       rdfs:comment "a Java regex the code or register notation must comply to." ;
                                       
                                       rdfs:subPropertyOf <http://metarelate.net/config/validationDataProperties> .



###  http://metarelate.net/config/pragmaDataProperty

<http://metarelate.net/config/pragmaDataProperty> rdf:type owl:DatatypeProperty .



###  http://metarelate.net/config/pragmaPad

<http://metarelate.net/config/pragmaPad> rdf:type owl:DatatypeProperty ;
                                         
                                         rdfs:comment """Specifies a pad value for index expansions.
E.g.: if entity/1-100 is expanded, and pragmaPad is 5, entities will be:
entity/00001, entity/00002 ...

(note, in some cases, auto padding is in use).""" ;
                                         
                                         rdfs:domain <http://metarelate.net/config/ExpandDashAndSuppress> ;
                                         
                                         rdfs:subPropertyOf <http://metarelate.net/config/pragmaDataProperty> .



###  http://metarelate.net/config/pseudoOrder

<http://metarelate.net/config/pseudoOrder> rdf:type owl:DatatypeProperty ;
                                           
                                           rdfs:comment "When more validation rules are provided, the system present a default input which includes properties that must or can be filled. The order of this input is determined by pseudo-order: properties are ordered (best effort) according to the strings associated via pseudoOrder." ;
                                           
                                           rdfs:domain <http://metarelate.net/config/ValidationTypes> ;
                                           
                                           rdfs:subPropertyOf <http://metarelate.net/config/validationDataProperties> .



###  http://metarelate.net/config/systemParameters

<http://metarelate.net/config/systemParameters> rdf:type owl:DatatypeProperty .



###  http://metarelate.net/config/validationDataProperties

<http://metarelate.net/config/validationDataProperties> rdf:type owl:DatatypeProperty .





#################################################################
#
#    Classes
#
#################################################################


###  http://metarelate.net/config/Action

<http://metarelate.net/config/Action> rdf:type owl:Class ;
                                      
                                      rdfs:subClassOf <http://metarelate.net/config/ProcessConfigurationTypes> ;
                                      
                                      rdfs:comment "an entity of this type is a valid action in the terminology management process (e.g.: validation, obsoletion...)" .



###  http://metarelate.net/config/AuthorizationSystem

<http://metarelate.net/config/AuthorizationSystem> rdf:type owl:Class .



###  http://metarelate.net/config/CodeValidationCommand

<http://metarelate.net/config/CodeValidationCommand> rdf:type owl:Class ;
                                                     
                                                     rdfs:subClassOf <http://metarelate.net/config/ValidationCommands> ;
                                                     
                                                     rdfs:comment "A comnand for the validation engine, regarding codes." .



###  http://metarelate.net/config/CodeValidationConstraint

<http://metarelate.net/config/CodeValidationConstraint> rdf:type owl:Class ;
                                                        
                                                        rdfs:subClassOf <http://metarelate.net/config/ValidationTypes> ;
                                                        
                                                        rdfs:comment "An entitity of this type defines a constraint for codes." .



###  http://metarelate.net/config/DataTypes

<http://metarelate.net/config/DataTypes> rdf:type owl:Class ;
                                         
                                         rdfs:subClassOf <http://metarelate.net/config/ValidationClasses> .



###  http://metarelate.net/config/ExpandDashAndSuppress

<http://metarelate.net/config/ExpandDashAndSuppress> rdf:type owl:Class ;
                                                     
                                                     rdfs:subClassOf <http://metarelate.net/config/Pragma> .



###  http://metarelate.net/config/ExpandTreeProcedure

<http://metarelate.net/config/ExpandTreeProcedure> rdf:type owl:Class ;
                                                   
                                                   rdfs:subClassOf <http://metarelate.net/config/Pragma> .



###  http://metarelate.net/config/Instance

<http://metarelate.net/config/Instance> rdf:type owl:Class ;
                                        
                                        rdfs:comment """An instance of the terminoloy manager
""" .



###  http://metarelate.net/config/Parameter

<http://metarelate.net/config/Parameter> rdf:type owl:Class ;
                                         
                                         rdfs:subClassOf <http://metarelate.net/config/PragmaOperators> .



###  http://metarelate.net/config/Pragma

<http://metarelate.net/config/Pragma> rdf:type owl:Class ;
                                      
                                      rdfs:subClassOf <http://metarelate.net/config/PragmaOperators> .



###  http://metarelate.net/config/PragmaOperators

<http://metarelate.net/config/PragmaOperators> rdf:type owl:Class .



###  http://metarelate.net/config/ProcessConfigurationTypes

<http://metarelate.net/config/ProcessConfigurationTypes> rdf:type owl:Class .



###  http://metarelate.net/config/PropertyFocus

<http://metarelate.net/config/PropertyFocus> rdf:type owl:Class .



###  http://metarelate.net/config/RegisterValidationCommand

<http://metarelate.net/config/RegisterValidationCommand> rdf:type owl:Class ;
                                                         
                                                         rdfs:subClassOf <http://metarelate.net/config/ValidationCommands> ;
                                                         
                                                         rdfs:comment "A comnand for the validation engine, regarding registers." .



###  http://metarelate.net/config/RegisterValidationConstraint

<http://metarelate.net/config/RegisterValidationConstraint> rdf:type owl:Class ;
                                                            
                                                            rdfs:subClassOf <http://metarelate.net/config/ValidationTypes> ;
                                                            
                                                            rdfs:comment "An entitity of this type defines a constraint for registers." .



###  http://metarelate.net/config/Role

<http://metarelate.net/config/Role> rdf:type owl:Class ;
                                    
                                    rdfs:subClassOf <http://metarelate.net/config/ProcessConfigurationTypes> ;
                                    
                                    rdfs:comment """Specifies a possible tranistion.
For a given action, one or more roles can be associated that express pre and post conditions for the state transition.""" .



###  http://metarelate.net/config/State

<http://metarelate.net/config/State> rdf:type owl:Class ;
                                     
                                     rdfs:subClassOf <http://metarelate.net/config/ProcessConfigurationTypes> ;
                                     
                                     rdfs:comment "An antity of this type is a valid state in the terminology management process (e.g.: obsolete, valid...)" .



###  http://metarelate.net/config/TerminologyEntity

<http://metarelate.net/config/TerminologyEntity> rdf:type owl:Class .



###  http://metarelate.net/config/ValidationClasses

<http://metarelate.net/config/ValidationClasses> rdf:type owl:Class .



###  http://metarelate.net/config/ValidationCommands

<http://metarelate.net/config/ValidationCommands> rdf:type owl:Class ;
                                                  
                                                  rdfs:subClassOf <http://metarelate.net/config/ValidationClasses> .



###  http://metarelate.net/config/ValidationTypes

<http://metarelate.net/config/ValidationTypes> rdf:type owl:Class ;
                                               
                                               rdfs:subClassOf <http://metarelate.net/config/ValidationClasses> .



###  http://metarelate.net/config/hardLimitCut

<http://metarelate.net/config/hardLimitCut> rdf:type owl:Class ;
                                            
                                            rdfs:subClassOf <http://metarelate.net/config/Parameter> ;
                                            
                                            rdfs:comment """When a max number of productions is specified, this property specify what should happen if the max number is reached.
E.g.: if a character is 1-100, we are in an expandDashAdnSuppress pragma, hardLimit is set to 20.
If hardLimit cut is not specified, only the entities 1,...,20 are going to be produced. Otherwise none will be produced. """ .



###  http://metarelate.net/config/pragmaSuppressSource

<http://metarelate.net/config/pragmaSuppressSource> rdf:type owl:Class ;
                                                    
                                                    rdfs:subClassOf <http://metarelate.net/config/Parameter> ;
                                                    
                                                    rdfs:comment "When entities like 1-10 are expanded in 1,...,10, the original entity is removed." .





#################################################################
#
#    Individuals
#
#################################################################


###  http://metarelate.net/config/Numeric

<http://metarelate.net/config/Numeric> rdf:type <http://metarelate.net/config/DataTypes> ,
                                                owl:NamedIndividual ;
                                       
                                       rdfs:comment "The object of the (data) property must be numeric (parses as Int)" .



###  http://metarelate.net/config/String

<http://metarelate.net/config/String> rdf:type <http://metarelate.net/config/DataTypes> ,
                                               owl:NamedIndividual ;
                                      
                                      rdfs:comment "the object of the (data) property must be a String." .



###  http://metarelate.net/config/allActions

<http://metarelate.net/config/allActions> rdf:type owl:NamedIndividual ;
                                          
                                          rdfs:comment """this individual specify a null constraints in authorization files:
<user> <action> <entity>
if <action> is allAction, this means the user can peroform all actions on the specified entity.""" .



###  http://metarelate.net/config/allActors

<http://metarelate.net/config/allActors> rdf:type owl:NamedIndividual ;
                                         
                                         rdfs:comment """this individual specify a null constraints in authorization files:
<user> <action> <entity>
if <actor> is allActor, this means any user can perform the specified action on the specified entity.""" .



###  http://metarelate.net/config/allEntities

<http://metarelate.net/config/allEntities> rdf:type owl:NamedIndividual ;
                                           
                                           rdfs:comment """this individual specify a null constraints in authorization files:
<user> <action> <entity>
if <entity> is allEntities, this means the user can peroform the specified action on all entities.""" .



###  http://metarelate.net/config/allRegisters

<http://metarelate.net/config/allRegisters> rdf:type <http://metarelate.net/config/TerminologyEntity> ,
                                                     owl:NamedIndividual ;
                                            
                                            rdfs:comment "Specifies all possible registers. As an object of the inRegister constraint, it specifies that the code must be known to the Terminology Manager. " .



###  http://metarelate.net/config/authIsInFile

<http://metarelate.net/config/authIsInFile> rdf:type owl:NamedIndividual ;
                                            
                                            rdfs:comment "Authorization via file" .



###  http://metarelate.net/config/clear

<http://metarelate.net/config/clear> rdf:type <http://metarelate.net/config/RegisterValidationCommand> ,
                                              owl:NamedIndividual ;
                                     
                                     rdfs:comment "For an individual and register, constraints are collected from all containing registers. The collection is bottom-up and stops if a \"clear\" command is associated to register (requests for constraints is not propagated upward of the register specified in the constraint)." .



###  http://metarelate.net/config/codeRelatedProperty

<http://metarelate.net/config/codeRelatedProperty> rdf:type <http://metarelate.net/config/PropertyFocus> ,
                                                            owl:NamedIndividual .



###  http://metarelate.net/config/conceptRelatedProperty

<http://metarelate.net/config/conceptRelatedProperty> rdf:type <http://metarelate.net/config/PropertyFocus> ,
                                                               owl:NamedIndividual .



###  http://metarelate.net/config/selfInstance

<http://metarelate.net/config/selfInstance> rdf:type <http://metarelate.net/config/Instance> ,
                                                     owl:NamedIndividual ;
                                            
                                            rdfs:comment "This instance represent the terminology system itself. A strange instance after all... but we are not in an ontology!" .




###  Generated by the OWL API (version 3.3.1957) http://owlapi.sourceforge.net

